qa/lean/Ragu/Instances/Element/Alloc.lean
@@ -5,33 +5,29 @@ import Ragu.Core
 namespace Ragu.Instances.Element.Alloc
 open Ragu.Instances.Autogen.Element.Alloc
 
-set_option linter.unusedVariables false in
-def deserializeInput (input : Vector (Expression (F p)) inputLen) : Var unit (F p) := ()
+def deserializeInput (_ : Vector (Expression (F p)) inputLen) :
+    Var (UnconstrainedDep Circuits.Core.AllocMul.Row) (F p) :=
+  fun _ => ⟨0, 0, 0⟩
 
 def serializeOutput (output : Var field (F p)) : Vector (Expression (F p)) 1 :=
   #v[output]
 
-def formal_instance : Core.Statements.GeneralFormalInstance where
+def formal_instance : Core.Statements.GeneralFormalWithHintInstance where
   p
   exportedOperations
   exportedOutput
-
-  Input := unit
-  Output := field
 
   deserializeInput
   serializeOutput
 
   Spec (_input : Unit) (_output : F p) := True
 
-  reimplementation :=
-    Circuits.Element.Alloc.circuit (fun _ => ⟨0, 0, 0⟩)
+  reimplementation := Circuits.Element.Alloc.circuit
 
   same_constraints := by
     intro input
     simp [Core.Statements.FlatOperation.eraseCompute, List.map,
       Operations.toFlat, circuit_norm,
-      GeneralFormalCircuit.toSubcircuit, GeneralFormalCircuit.toWithHint,
       GeneralFormalCircuit.WithHint.toSubcircuit,
       deserializeInput, exportedOperations,
       Circuits.Element.Alloc.circuit,
@@ -44,7 +40,6 @@ def formal_instance : Core.Statements.GeneralFormalInstance where
   same_output := by
     intro input
     simp [circuit_norm,
-      GeneralFormalCircuit.toSubcircuit, GeneralFormalCircuit.toWithHint,
       GeneralFormalCircuit.WithHint.toSubcircuit,
       deserializeInput, serializeOutput,
       Circuits.Element.Alloc.circuit,
