qa/lean/Ragu/Instances/Element/AllocSquare.lean
@@ -6,31 +6,29 @@ namespace Ragu.Instances.Element.AllocSquare
 open Ragu.Instances.Autogen.Element.AllocSquare
 
 set_option linter.unusedVariables false in
-def deserializeInput (input : Vector (Expression (F p)) inputLen) : Var unit (F p) := ()
+def deserializeInput (input : Vector (Expression (F p)) inputLen) :
+    Var (UnconstrainedDep field) (F p) :=
+  fun _ => 0
 
 def serializeOutput (output : Var Circuits.Element.AllocSquare.Square (F p)) : Vector (Expression (F p)) 2 :=
   #v[output.a, output.a_sq]
 
-def formal_instance : Core.Statements.GeneralFormalInstance where
+def formal_instance : Core.Statements.GeneralFormalWithHintInstance where
   p
   exportedOperations
   exportedOutput
-
-  Input := unit
-  Output := Circuits.Element.AllocSquare.Square
 
   deserializeInput
   serializeOutput
 
   Spec _input output := output.a_sq = output.a^2
 
-  reimplementation := Circuits.Element.AllocSquare.circuit (fun _ => 0)
+  reimplementation := Circuits.Element.AllocSquare.circuit
 
   same_constraints := by
     intro input
     simp [Core.Statements.FlatOperation.eraseCompute, List.map,
       Operations.toFlat, circuit_norm,
-      GeneralFormalCircuit.toSubcircuit, GeneralFormalCircuit.toWithHint,
       GeneralFormalCircuit.WithHint.toSubcircuit,
       deserializeInput, exportedOperations,
       Circuits.Element.AllocSquare.circuit,
@@ -44,7 +42,6 @@ def formal_instance : Core.Statements.GeneralFormalInstance where
   same_output := by
     intro input
     simp [circuit_norm,
-      GeneralFormalCircuit.toSubcircuit, GeneralFormalCircuit.toWithHint,
       GeneralFormalCircuit.WithHint.toSubcircuit,
       deserializeInput, serializeOutput,
       Circuits.Element.AllocSquare.circuit,
