qa/lean/Ragu/Instances/Element/Invert.lean
@@ -5,33 +5,27 @@ import Ragu.Core
 namespace Ragu.Instances.Element.Invert
 open Ragu.Instances.Autogen.Element.Invert
 
-def deserializeInput (input : Vector (Expression (F p)) inputLen) : Var field (F p) :=
-  input[0]
+def deserializeInput (input : Vector (Expression (F p)) inputLen) :
+    Var Circuits.Element.Invert.Input (F p) :=
+  { input := input[0], hint := fun _ => ⟨0, 0, 0⟩ }
 
 def serializeOutput (output : Var field (F p)) : Vector (Expression (F p)) 1 :=
   #v[output]
 
-def formal_instance : Core.Statements.GeneralFormalInstance where
+def formal_instance : Core.Statements.GeneralFormalWithHintInstance where
   p
   exportedOperations
   exportedOutput
 
-  Input := field
-  Output := field
-
   deserializeInput
   serializeOutput
 
-  Spec (input : F p) (output : F p) := input * output = 1
-
-  reimplementation :=
-    Circuits.Element.Invert.circuit (fun _ => ⟨0, 0, 0⟩)
+  reimplementation := Circuits.Element.Invert.circuit
 
   same_constraints := by
     intro input
     simp [Core.Statements.FlatOperation.eraseCompute, List.map,
       Operations.toFlat, circuit_norm,
-      GeneralFormalCircuit.toSubcircuit, GeneralFormalCircuit.toWithHint,
       GeneralFormalCircuit.WithHint.toSubcircuit,
       deserializeInput, exportedOperations,
       Circuits.Element.Invert.circuit,
@@ -48,7 +42,6 @@ def formal_instance : Core.Statements.GeneralFormalInstance where
   same_output := by
     intro input
     simp [circuit_norm,
-      GeneralFormalCircuit.toSubcircuit, GeneralFormalCircuit.toWithHint,
       GeneralFormalCircuit.WithHint.toSubcircuit,
       deserializeInput, serializeOutput,
       Circuits.Element.Invert.circuit,
@@ -60,10 +53,5 @@ def formal_instance : Core.Statements.GeneralFormalInstance where
       Circuits.Core.AllocMul.circuit,
       Circuits.Core.AllocMul.elaborated,
       Circuits.Core.AllocMul.main]
-  same_spec := by
-    intro input output
-    dsimp only [Circuits.Element.Invert.circuit,
-      Circuits.Element.Invert.Spec]
-    aesop
 
 end Ragu.Instances.Element.Invert
